adding push pop semantics

theory/rBPFCommType.thy
@@ -119,24 +119,29 @@ definition u8_list_of_u64 :: "u64 \<Rightarrow> u8 list" where
     (ucast (i >> 56))
   ]"
 
-fun ua_of_u8_list_aux :: "u8 list \<Rightarrow> 'a :: len word" where
-"ua_of_u8_list_aux [] = 0" |
-"ua_of_u8_list_aux (h#t) = or (ucast h) ((ua_of_u8_list_aux t) << 8)"
+fun ua_of_u8_list_aux :: "u8 list \<Rightarrow> ('a :: len word) option" where
+"ua_of_u8_list_aux [] = None" |
+"ua_of_u8_list_aux [h] = Some (ucast h)" |
+"ua_of_u8_list_aux (h#t) = (
+  case ua_of_u8_list_aux t of
+  None \<Rightarrow> None |
+  Some v \<Rightarrow> Some (or (ucast h) (v << 8))
+)"
 
-definition u64_of_u8_list :: "u8 list \<Rightarrow> u64" where
-"u64_of_u8_list l = ua_of_u8_list_aux (rev l)"
+definition u64_of_u8_list :: "u8 list \<Rightarrow> u64 option" where
+"u64_of_u8_list l = (if length l = 8 then ua_of_u8_list_aux (rev l) else None)"
 
-definition u32_of_u8_list :: "u8 list \<Rightarrow> u32" where
-"u32_of_u8_list l = ua_of_u8_list_aux (rev l)"
+definition u32_of_u8_list :: "u8 list \<Rightarrow> u32 option" where
+"u32_of_u8_list l = (if length l = 4 then ua_of_u8_list_aux (rev l) else None)"
 
-definition u16_of_u8_list :: "u8 list \<Rightarrow> u16" where
-"u16_of_u8_list l = ua_of_u8_list_aux (rev l)"
+definition u16_of_u8_list :: "u8 list \<Rightarrow> u16 option" where
+"u16_of_u8_list l = (if length l = 2 then ua_of_u8_list_aux (rev l) else None)"
 
 
 lemma [simp]: "u8_of_bool False = 0" by (unfold u8_of_bool_def, simp)
 
 lemma [simp]: "u8_of_bool True = 1" by (unfold u8_of_bool_def, simp)
 
-lemma [simp]: "u8_list_of_u64 (u64_of_u8_list (l::u8 list)) = l "  sorry
+lemma [simp]: "(u64_of_u8_list l = Some v) = (u8_list_of_u64 v = l)" sorry
 
 end
