theory/Mem.thy
@@ -16,5 +16,13 @@ axiomatization
   loadv   :: "memory_chunk \<Rightarrow> mem \<Rightarrow> addr_type \<Rightarrow> val option" and
   storev  :: "memory_chunk \<Rightarrow> mem \<Rightarrow> addr_type \<Rightarrow> val \<Rightarrow> mem option"
 
+definition vlong_of_memory_chunk :: "memory_chunk \<Rightarrow> val" where
+"vlong_of_memory_chunk chunk = (
+  case chunk of
+  M8  \<Rightarrow> Vlong 8 |
+  M16 \<Rightarrow> Vlong 16 |
+  M32 \<Rightarrow> Vlong 32 |
+  M64 \<Rightarrow> Vlong 64
+)"
 
 end
